Finalize GhostDAG total

Ghostdag.thy
@@ -64,9 +64,8 @@ function OrderDAG :: "('a::linorder,'b) pre_digraph \<Rightarrow> nat \<Rightarr
   if (card (verts G) = 1)  then ({genesis_nodeAlt G},[genesis_nodeAlt G]) else
  let M =  choose_max_blue_set 
   ((map (\<lambda>i.(((OrderDAG (reduce_past G i) k)) , i)) (sorted_list_of_set (tips G))))
- in let Current = (add_set_list_tuple M, snd M)
  in fold (app_if_blue_else_add_end G k) (top_sort G (sorted_list_of_set (anticone G (snd M))))
- (fst Current))
+ (add_set_list_tuple M))
  "
   by auto
 termination proof 
@@ -91,6 +90,13 @@ next
     by fastforce  
 qed
 
+lemma add_set_list_tuple_mono:
+  shows "set L \<subseteq> set (snd (add_set_list_tuple ((S,L),a)))"
+  using add_set_list_tuple.simps by auto
+
+lemma add_set_list_tuple_mono2:
+  shows "set (snd (add_set_list_tuple ((S,L),a))) \<subseteq> set L \<union> {a} "
+  using add_set_list_tuple.simps by auto
 
 lemma app_if_blue_mono:
   assumes "finite S"
@@ -104,11 +110,23 @@ lemma app_if_blue_mono2:
   by (simp add: subsetI)
 
 
-
 lemma app_if_blue_append:
   shows  "a \<in> set (snd (app_if_blue_else_add_end G k a (S,L) ))"
   unfolding app_if_blue_else_add_end.simps add_set_list_tuple.simps
   by simp
+
+lemma app_if_blue_mono3:
+  shows  "set (snd (app_if_blue_else_add_end G k a (S,L))) \<subseteq> set L \<union> {a}"
+  unfolding app_if_blue_else_add_end.simps add_set_list_tuple.simps
+  by (simp add: subsetI)
+
+lemma app_if_blue_mono4:
+  assumes "set L1 \<subseteq> set L2"
+  shows  "set (snd (app_if_blue_else_add_end G k a (S,L1)))
+   \<subseteq> set (snd (app_if_blue_else_add_end G k a (S2,L2)))"
+  unfolding app_if_blue_else_add_end.simps add_set_list_tuple.simps
+  using assms by auto
+ 
 
 lemma app_if_blue_card_mono:
   assumes "finite S"
@@ -145,10 +163,10 @@ proof (rule fold_invariant)
 
 lemma fold_app_mono:
   assumes "x \<in> set (snd (S,L1))"
-  shows " x \<in> set (snd (fold (app_if_blue_else_add_end G k) L2 (S,L1)))"
+  shows " x \<in> set (snd (fold (app_if_blue_else_add_end G k) L2 (S2,L1)))"
 proof(rule fold_invariant)
   show "\<And>x. x \<in> set L2 \<Longrightarrow>  x \<in> set L2" by simp
-  show "x \<in> set (snd (S, L1))" using assms(1) by simp
+  show "x \<in> set (snd (S2, L1))" using assms(1) by simp
   show "\<And>xa s. xa \<in> set L2 \<Longrightarrow> x \<in> set (snd s) \<Longrightarrow> 
   x \<in> set (snd (app_if_blue_else_add_end G k xa s)) " by auto 
 qed  
@@ -204,28 +222,58 @@ next
   qed
 qed
 
+lemma fold_app_mono_ex: 
+ shows "(set L2 \<union> set L1) = set (snd (fold (app_if_blue_else_add_end G k) L2 (S,L1)))" 
+proof
+  show "set L2 \<union> set L1 \<subseteq> set (snd (fold (app_if_blue_else_add_end G k) L2 (S, L1)))"
+    using fold_app_mono fold_app_mono2 by auto
+next
+  show "set (snd (fold (app_if_blue_else_add_end G k) L2 (S, L1))) \<subseteq> set L2 \<union> set L1" 
+  proof(rule fold_invariant)
+      show "\<And>x. x \<in> set L2 \<Longrightarrow>  x \<in> set L2" by auto
+    next 
+      show "set (snd (S, L1)) \<subseteq> set L2 \<union> set L1" by auto
+    next 
+      fix x 
+      fix s::"'a set \<times> 'a list" 
+      assume x_in: "x \<in> set L2"
+      and s_sub: "set (snd s) \<subseteq> set L2 \<union> set L1"
+      then have "set (snd (app_if_blue_else_add_end G k x s)) \<subseteq> 
+      set (snd (app_if_blue_else_add_end G k x (fst s, L2 @ L1)))"
+        using app_if_blue_mono4
+        by (metis prod.collapse set_append)
+      then show "set (snd (app_if_blue_else_add_end G k x s)) \<subseteq> set L2 \<union> set L1" 
+        using x_in app_if_blue_mono3
+        by fastforce
+    qed
+  qed
+
 lemma (in tie_breakingDAG) OrderDAG_total: 
-  shows "x \<in> verts G \<longrightarrow> x \<in> set (snd (OrderDAG G k))" 
-proof(safe)
-  have bD: "blockDAG G" using tie_breakingDAG_axioms tie_breakingDAG_def by auto
+  shows "x \<in> verts G \<longrightarrow> x \<in> set (snd (OrderDAG G k))"
+  using tie_breakingDAG_axioms
+proof(safe, induct G k  arbitrary: x rule: OrderDAG.induct)
+  case (1 G k x)
+  then have bD: "blockDAG G" using tie_breakingDAG_axioms tie_breakingDAG_def by auto
   assume x_in: "x \<in> verts G"
   then consider (cD1) "card (verts G) = 1"| (cDm) "card (verts G) \<noteq> 1" by auto 
   then show "x \<in> set (snd (OrderDAG G k))"
   proof(cases)
     case (cD1)
     then have "set (snd (OrderDAG G k)) = {genesis_nodeAlt G}" 
-      using tie_breakingDAG_axioms OrderDAG.simps by auto
+      using 1 OrderDAG.simps by auto
     then show ?thesis using x_in bD cD1
          genesis_nodeAlt_sound blockDAG.is_genesis_node.simps
-      using gen_gen gen_graph_all_one by fastforce 
+      using gen_gen gen_graph_all_one 1
+      by (metis card_1_singletonE singletonD) 
   next
     case (cDm)
     then show ?thesis
     proof -
       obtain pp where pp_in: "pp =  (map (\<lambda>i. (OrderDAG (reduce_past G i) k, i))
        (sorted_list_of_set (tips G)))" using tips_exist by auto
-      have mm: "choose_max_blue_set pp \<in> set pp" using pp_in choose_max_blue_avoid_empty tips_finite
-         list.map_disc_iff sorted_list_of_set_eq_Nil_iff tips_not_empty
+      have mm: "choose_max_blue_set pp \<in> set pp" using pp_in choose_max_blue_avoid_empty
+          digraph.tips_finite subs 1 bD 
+         list.map_disc_iff sorted_list_of_set_eq_Nil_iff blockDAG.tips_not_empty 
         by (metis (mono_tags, lifting))  
       then have kk: "snd (choose_max_blue_set pp) \<in> set (map  snd pp)"
         by auto 
@@ -244,7 +292,7 @@ proof(safe)
       have "set (map snd pp) = set (sorted_list_of_set (tips G))" 
         using mm2 pp_in  by auto
       then have tt2: "snd (choose_max_blue_set pp) \<in> tips G"
-        using tips_finite sorted_list_of_set(1) kk  by auto  
+        using digraph.tips_finite sorted_list_of_set(1) kk bD subs  by auto  
       show ?thesis 
          proof(rule blockDAG.tips_cases)
          show "blockDAG G" using bD by auto
@@ -252,62 +300,154 @@ proof(safe)
          show "x \<in> verts G" using x_in by auto
        next  
         assume as1: "x = snd (choose_max_blue_set pp)"
-        obtain Cur where cur_in: "Cur = fst (add_set_list_tuple (choose_max_blue_set pp), x)"
+        obtain fCur where fcur_in: "fCur = add_set_list_tuple (choose_max_blue_set pp)"
             by auto
-        have "x \<in> set (snd(Cur))" 
-          unfolding as1 using  add_set_list_tuple.simps cur_in
+        have "x \<in> set (snd(fCur))" 
+          unfolding as1 using  add_set_list_tuple.simps fcur_in
           add_set_list_tuple.cases snd_conv insertI1 snd_conv
           by (metis (mono_tags, hide_lams) Un_insert_right fst_conv list.simps(15) set_append) 
         then have "x \<in> set (snd (fold (app_if_blue_else_add_end G k)
-                   (top_sort G (sorted_list_of_set (anticone G (snd (choose_max_blue_set pp))))) (Cur)))"
+                   (top_sort G (sorted_list_of_set (anticone G (snd (choose_max_blue_set pp))))) (fCur)))"
           using  finite_verts fold_app_mono surj_pair
         by (metis)
-      then show ?thesis unfolding pp_in cur_in using tie_breakingDAG_axioms OrderDAG.simps cDm
-         fst_conv 
+      then show ?thesis unfolding pp_in fcur_in using 1 OrderDAG.simps cDm
         by (metis (mono_tags, lifting)) 
       next
         assume anti: "x \<in> anticone G (snd (choose_max_blue_set pp))" 
-        obtain ttt where ttt_in: "ttt = fst (add_set_list_tuple (choose_max_blue_set pp)
-        , snd (choose_max_blue_set pp))" by auto
+        obtain ttt where ttt_in: "ttt = add_set_list_tuple (choose_max_blue_set pp)" by auto
         have "x \<in> set (snd (fold (app_if_blue_else_add_end G k)
                  (top_sort G (sorted_list_of_set (anticone G (snd (choose_max_blue_set pp)))))
                    ttt))" 
-          using pp_in sorted_list_of_set(1) anti
-         anticon_finite fold_app_mono2 surj_pair top_sort_con  by metis 
-        then show "x \<in> set (snd (OrderDAG G k))" using OrderDAG.simps pp_in bD cDm ttt_in 
-          by (metis (no_types, lifting) map_eq_conv tie_breakingDAG_axioms) 
+          using pp_in sorted_list_of_set(1) anti bD subs
+         DAG.anticon_finite fold_app_mono2 surj_pair top_sort_con  by metis 
+        then show "x \<in> set (snd (OrderDAG G k))" using OrderDAG.simps pp_in bD cDm ttt_in 1
+          by (metis (no_types, lifting) map_eq_conv) 
       next 
         assume  as2: "x \<in> past_nodes G (snd (choose_max_blue_set pp))"
-        show "x \<in> set (snd (OrderDAG G k))" using tie_breakingDAG_axioms pp_in
-          
-        
-
-
-(*
-proof (safe, induction G rule: blockDAG_induct)
-  case fund
-  then show ?case using tie_breakingDAG_def tie_breakingDAG_axioms by auto
-next 
-  case (base V)
-  then have cD: "card (verts (blockDAG.gen_graph V)) = 1" using blockDAG.gen_graph_one by simp 
-  have tB: "tie_breakingDAG ((blockDAG.gen_graph V)) \<and> blockDAG ((blockDAG.gen_graph V)) "
-    using tie_breakingDAG_def base.hyps blockDAG.gen_graph_sound by auto
-  then have res: " set (snd (OrderDAG (blockDAG.gen_graph V) k)) 
-  = {genesis_nodeAlt (blockDAG.gen_graph V)}"
-  using OrderDAG.simps cD by auto
-  assume x_in: "x \<in> verts (blockDAG.gen_graph V)"
-  then have "blockDAG.is_genesis_node (blockDAG.gen_graph V) x"
-    by (metis blockDAG.no_empty_blockDAG blockDAG.reduce_less blockDAG.reduce_past_dagbased
-        cD gr_implies_not0 less_one tB)
-  then have "genesis_nodeAlt (blockDAG.gen_graph V) = x"
-    by (metis blockDAG.genesis_unique_exists cD genesis_nodeAlt_one_sound tB) 
-  then show "x \<in> set (snd (OrderDAG (blockDAG.gen_graph V) k))"
-    using res genesis_nodeAlt_sound tB blockDAG.unique_genesis
-    by auto 
-next
-  case (step H)
-  then show ?case 
+        then have pas: "x \<in> verts (reduce_past G (snd (choose_max_blue_set pp)))" 
+          using reduce_past.simps induce_subgraph_verts by auto
+        have cd1: "card (verts G) > 1" using cDm bD
+          using blockDAG.blockDAG_size_cases by blast 
+        have "(snd (choose_max_blue_set pp)) \<in> set (sorted_list_of_set (tips G))" using tt2
+        digraph.tips_finite bD subs sorted_list_of_set(1) by auto
+        moreover 
+        have "tie_breakingDAG (reduce_past G (snd (choose_max_blue_set pp)))" using 
+        blockDAG.reduce_past_dagbased bD tt2  blockDAG.tips_unequal_gen 
+        cd1 tie_breakingDAG_def tips_def CollectD by metis
+        ultimately have bass: 
+          "x \<in> set ((snd (OrderDAG (reduce_past G (snd (choose_max_blue_set pp))) k)))" 
+          using  pp_in 1 cDm tt2 pas by metis
+        then have in_F: "x \<in> set (snd ( fst ((choose_max_blue_set pp))))" unfolding pp_in
+          using surj_pair
+          imageE list.set_map mm old.prod.inject pp_in prod.collapse
+          by (smt (verit, best))
+        then have "x \<in> set (snd (fst (choose_max_blue_set pp)))"
+          using pp_in
+          by (metis (no_types, lifting)) 
+        then have "x \<in> set (snd (fold (app_if_blue_else_add_end G k)
+         (top_sort G (sorted_list_of_set (anticone G (snd (choose_max_blue_set pp)))))
+         (fst((choose_max_blue_set pp)))))"
+          by (metis fold_app_mono in_F prod.collapse) 
+        moreover have "OrderDAG G k = (fold (app_if_blue_else_add_end G k)
+         (top_sort G (sorted_list_of_set (anticone G (snd (choose_max_blue_set pp)))))
+         (add_set_list_tuple (choose_max_blue_set pp)))" using cDm 1(4) OrderDAG.simps pp_in
+          by (metis (no_types, lifting) map_eq_conv) 
+        then show "x \<in> set (snd (OrderDAG G k))"
+          by (metis (no_types, lifting) add_set_list_tuple_mono fold_app_mono
+               in_F prod.collapse subset_code(1))  
+      qed
+    qed
+  qed
 qed
-*)
+
+
+lemma "x \<in> set (snd (OrderDAG G k)) \<longrightarrow> x \<in> verts G"
+proof(induction G k arbitrary: x rule: OrderDAG.induct)
+  case (1 G k x)
+  consider (inval) "\<not> tie_breakingDAG G"| (one) "tie_breakingDAG G \<and>
+  card (verts G) = 1" | (val) "tie_breakingDAG G \<and>
+  card (verts G) \<noteq> 1" by auto
+  then show ?case 
+  proof(cases)
+    case inval
+    then show ?thesis using OrderDAG.simps by auto
+  next
+    case one
+    then show ?thesis using OrderDAG.simps genesis_nodeAlt_one_sound blockDAG.is_genesis_node.simps
+    tie_breakingDAG_def
+      using empty_set list.simps(15) singleton_iff sndI by fastforce  
+  next
+    case val
+    then show ?thesis
+    proof safe
+    have bD: "blockDAG G" using val tie_breakingDAG_def by auto
+    assume pre: "x \<in> set (snd (OrderDAG G k))"
+    obtain M where M_in:"M = choose_max_blue_set (map (\<lambda>i. (OrderDAG (reduce_past G i) k, i))
+       (sorted_list_of_set (tips G)))" by auto
+      obtain pp where pp_in: "pp =  (map (\<lambda>i. (OrderDAG (reduce_past G i) k, i))
+       (sorted_list_of_set (tips G)))" using blockDAG.tips_exist by auto
+          have mm: "choose_max_blue_set pp \<in> set pp" using pp_in choose_max_blue_avoid_empty
+              digraph.tips_finite subs 1 bD 
+             list.map_disc_iff sorted_list_of_set_eq_Nil_iff blockDAG.tips_not_empty 
+            by (metis (mono_tags, lifting))  
+          then have kk: "snd (choose_max_blue_set pp) \<in> set (map  snd pp)"
+            by auto 
+          have mm2: "\<And>L. (map snd (map (\<lambda>i. ((OrderDAG (reduce_past G i) k) , i)) L)) =  L" 
+          proof -
+            fix L
+            show "map snd (map (\<lambda>i. (OrderDAG (reduce_past G i) k, i)) L) = L"
+            proof(induct L)
+              case Nil
+              then show ?case by auto
+            next
+              case (Cons a L)
+              then show ?case by auto
+            qed
+          qed
+          have "set (map snd pp) = set (sorted_list_of_set (tips G))" 
+            using mm2 pp_in  by auto
+          then have tt2: "snd (choose_max_blue_set pp) \<in> tips G"
+            using digraph.tips_finite sorted_list_of_set(1) kk bD subs  by auto
+      have "set (snd (OrderDAG G k)) =
+       set (snd (fold (app_if_blue_else_add_end G k) (top_sort G (sorted_list_of_set (anticone G (snd M))))
+      (add_set_list_tuple M)))" unfolding M_in val using OrderDAG.simps val
+        by (metis (mono_tags, lifting)) 
+      then have "set (snd (OrderDAG G k)) 
+    = set (top_sort G (sorted_list_of_set (anticone G (snd M)))) \<union> set (snd (add_set_list_tuple M))"
+        using fold_app_mono_ex
+        by (metis eq_snd_iff)
+    then consider (ac) "x \<in> set (top_sort G (sorted_list_of_set (anticone G (snd M))))" 
+        | (co) "x \<in> set (snd (add_set_list_tuple M))" 
+      using pre by auto
+    then show "x \<in> verts G" proof(cases)
+        case ac
+        then show ?thesis using top_sort_con DAG.anticone_in_verts val tie_breakingDAG_def 
+        sorted_list_of_set(1) subs
+          by (metis DAG.anticon_finite subsetD) 
+      next
+        case co
+        then consider (ma) "x = snd M" | (nma) "x \<in> set (snd( fst(M)))" 
+          using add_set_list_tuple.simps
+          by (metis (no_types, lifting) Un_insert_right append_Nil2 insertE
+              list.simps(15) prod.collapse set_append sndI) 
+        then show ?thesis proof(cases)
+          case ma
+          then show ?thesis unfolding M_in  using pp_in M_in ma digraph.tips_in_verts bD subs tt2
+            by auto
+        next
+          case nma
+          then have "x \<in> set (snd (OrderDAG (reduce_past G (snd M)) k))" 
+            unfolding M_in choose_max_blue_avoid_empty blockDAG.tips_not_empty bD
+            by (metis (no_types, lifting) ex_map_conv fst_conv mm pp_in snd_conv) 
+          then have "x \<in> verts (reduce_past G (snd M))" using 1 val tt2 M_in pp_in 
+          sorted_list_of_set(1) digraph.tips_finite subs bD
+            by blast 
+          then show "x \<in> verts G" using reduce_past.simps induce_subgraph_verts past_nodes.simps
+            by auto
+        qed
+      qed 
+    qed
+  qed
+qed
 
 end
